Make progress with known correctness
Have to use "strict submap" over globals approximation map, and this in
turn is going to require that expressions only ever have one call to
SetGlobal n for each n. Already established that this is OK.

Working through the knock-on effects, all of which seem doable.

compiler/backend/proofs/clos_knownProofScript.sml
@@ -38,6 +38,67 @@ val error_case_eq =
                       nchotomy = error_CASES}
 
 (* MOVE candidates *)
+fun nailIHx k = let
+  fun hdt t = (t |> lhs |> strip_comb |> #1)
+              handle HOL_ERR _ => t |> strip_comb |> #1
+  fun sameish t1 t2 = aconv t1 t2 orelse same_const t1 t2
+  fun samehd t1 th2 = sameish (hdt t1) (hdt (concl th2))
+  fun findcs [] a k = raise Fail "strip_conj gave empty list"
+    | findcs [c] a k =
+      first_assum
+        (fn th => k (LIST_CONJ (List.rev (assert (samehd c) th :: a))))
+    | findcs (c::cs) a k =
+      first_assum (fn th => findcs cs (assert (samehd c) th :: a) k)
+in
+  first_x_assum
+    (fn th0 =>
+        let val body = th0 |> concl |> strip_forall |> #2
+            val hyp = #1 (dest_imp body)
+            val cs = strip_conj hyp
+        in
+          findcs cs [] (k o MATCH_MP th0)
+        end)
+end
+
+fun avSPEC_ALL avds th =
+  let
+    fun recurse avds acc th =
+      case Lib.total dest_forall (concl th) of
+          SOME (v,bod) =>
+          let
+            val v' = variant avds v
+          in
+            recurse (v'::avds) (v'::acc) (SPEC v' th)
+          end
+        | NONE => (List.rev acc, th)
+  in
+    recurse avds [] th
+  end
+
+fun PART_MATCH' f th t =
+  let
+    val (vs, _) = strip_forall (concl th)
+    val hypfvs_set = hyp_frees th
+    val hypfvs = HOLset.listItems hypfvs_set
+    val tfvs = free_vars t
+    val dontspec = union tfvs hypfvs
+    val (vs, speccedth) = avSPEC_ALL dontspec th
+    val ((tmsig,_),_) = raw_match [] hypfvs_set (f (concl speccedth)) t ([],[])
+    val dontgen = union (map #redex tmsig) dontspec
+  in
+    GENL (set_diff vs dontgen) (INST tmsig speccedth)
+  end
+
+fun asmPART_MATCH' f th t =
+    PART_MATCH' (f o strip_conj o #1 o dest_imp) th t
+
+fun sel_ihpc f =
+    first_assum (fn asm => first_x_assum (fn ih =>
+      mp_tac (asmPART_MATCH' f ih (concl asm))))
+
+fun resolve_selected f th =
+  first_assum (mp_tac o asmPART_MATCH' f th o concl)
+
 val _ = export_rewrites ["closLang.exp_size_def"]
 
 val any_el_ALT = Q.store_thm(
@@ -152,26 +213,111 @@ val safe_opsetg_def = Define`
          ∃a. args = [a] ∧ no_top_getGlobal a)
 `;
 
-val safe_setglobals_def = tDefine "safe_setglobals" `
-  (safe_setglobals (Var _) = T) ∧
-  (safe_setglobals (If e1 e2 e3) ⇔
-     safe_setglobals e1 ∧ safe_setglobals e2 ∧ safe_setglobals e3) ∧
-  (safe_setglobals (Let bs e) ⇔
-     (∀b. MEM b bs ⇒ safe_setglobals b) ∧ safe_setglobals e) ∧
-  (safe_setglobals (Raise e) = safe_setglobals e) ∧
-  (safe_setglobals (Handle e1 e2) ⇔ safe_setglobals e1 ∧ safe_setglobals e2) ∧
-  (safe_setglobals (Tick e) = safe_setglobals e) ∧
-  (safe_setglobals (Call _ es) = ∀e. MEM e es ⇒ safe_setglobals e) ∧
-  (safe_setglobals (App _ f args) ⇔
-    safe_setglobals f ∧ ∀a. MEM a args ⇒ safe_setglobals a) ∧
-  (safe_setglobals (Fn _ _ _ b) = safe_setglobals b) ∧
-  (safe_setglobals (Letrec _ _ bs b) ⇔
-    (∀n e. MEM (n,e) bs ⇒ safe_setglobals e) ∧ safe_setglobals b) ∧
-  (safe_setglobals (Op opn args) ⇔
-    ∀n a. opn = SetGlobal n ∧ MEM a args ⇒ no_top_getGlobal a)
-` (WF_REL_TAC `measure exp_size` >> simp[] >> rpt strip_tac >>
+val op_gbag_def = Define`
+  op_gbag (SetGlobal n) = BAG_INSERT n {||} ∧
+  op_gbag _ = {||}
+`;
+
+val set_globals_def = tDefine "set_globals" `
+  (set_globals (Var _) = {||}) ∧
+  (set_globals (If e1 e2 e3) =
+    set_globals e1 ⊎ set_globals e2 ⊎ set_globals e3) ∧
+  (set_globals (Let binds e) =
+    FOLDR $BAG_UNION (set_globals e) (MAP set_globals binds)) ∧
+  (set_globals (Raise e) = set_globals e) ∧
+  (set_globals (Handle e1 e2) = set_globals e1 ⊎ set_globals e2) ∧
+  (set_globals (Tick e) = set_globals e) ∧
+  (set_globals (Call _ args) = FOLDR $BAG_UNION {||} (MAP set_globals args)) ∧
+  (set_globals (App _ f args) =
+    FOLDR $BAG_UNION (set_globals f) (MAP set_globals args)) ∧
+  (set_globals (Fn _ _ _ bod) = set_globals bod) ∧
+  (set_globals (Letrec _ _ fbinds bod) =
+    FOLDR (λne s. set_globals (SND ne) ⊎ s) (set_globals bod) fbinds) ∧
+  (set_globals (Op opn args) =
+    FOLDR $BAG_UNION (op_gbag opn) (MAP set_globals args))
+`
+  (WF_REL_TAC `measure exp_size` >> simp[] >> rpt strip_tac >>
    imp_res_tac exp_size_MEM >> simp[])
 
+val elist_globals_def = Define`
+  elist_globals es = FOLDR BAG_UNION {||} (MAP set_globals es)
+`;
+val elist_globals_thm = Q.store_thm(
+  "elist_globals_thm[simp]",
+  `elist_globals [] = {||} ∧
+   elist_globals (exp::rest) = set_globals exp ⊎ elist_globals rest`,
+  simp[elist_globals_def]);
+
+val FOLDR_BAG_UNION_extract_acc = Q.store_thm(
+  "FOLDR_BAG_UNION_extract_acc",
+  `∀l a b. a ⊎ FOLDR (BAG_UNION o f) b l = FOLDR (BAG_UNION o f) (a ⊎ b) l`,
+  Induct_on `l` >> simp[] >> metis_tac[COMM_BAG_UNION, ASSOC_BAG_UNION])
+val foldr_bu =
+    FOLDR_BAG_UNION_extract_acc |> SPEC_ALL
+                                |> INST_TYPE [alpha |-> ``:β bag``]
+                                |> Q.INST [`b` |-> `{||}`, `f` |-> `I`]
+                                |> SIMP_RULE (srw_ss()) []
+                                |> GSYM
+
+val foldr_bu' =
+    FOLDR_BAG_UNION_extract_acc |> SPEC_ALL
+                                |> Q.INST [`b` |-> `{||}`, `f` |-> `λa. g a`]
+                                |> SIMP_RULE (srw_ss()) [o_ABS_R]
+                                |> GSYM
+
+
+val set_globals_def = save_thm("set_globals_def[simp]",
+  set_globals_def |> ONCE_REWRITE_RULE [foldr_bu]
+                  |> SIMP_RULE (srw_ss() ++ ETA_ss) [GSYM elist_globals_def])
+val set_globals_ind = theorem "set_globals_ind"
+
+val known_changed_globals = Q.store_thm(
+  "known_changed_globals",
+  `∀es as g0 alist g.
+     known es as g0 = (alist, g) ⇒
+     ∀i. i ∈ domain g ∧ (i ∈ domain g0 ⇒ lookup i g ≠ lookup i g0) ⇒
+         i ∈ SET_OF_BAG (elist_globals es)`,
+  ho_match_mp_tac known_ind >> simp[known_def] >> rpt strip_tac >>
+  rpt (pairarg_tac >> fs[]) >> rveq >> fs[]
+  >- (map_every qcase_tac [`known [exp1] as g0 = (al,g')`,`i ∈ domain g`] >>
+      Cases_on `i ∈ domain g'` >> fs[] >>
+      Cases_on `i ∈ domain g0` >> fs[] >>
+      Cases_on `lookup i g' = lookup i g0` >> fs[])
+  >- (map_every qcase_tac [
+        `known [exp1] as g0 = (al1,g1)`,
+        `known [exp2] as g1 = (al2,g2)`,
+        `known [exp3] as g2 = (al3,g3)`] >>
+      Cases_on `i ∈ domain g2` >> fs[] >>
+      Cases_on `i ∈ domain g1` >> fs[] >>
+      Cases_on `i ∈ domain g0` >> fs[] >>
+      Cases_on `lookup i g1 = lookup i g0` >> fs[] >>
+      Cases_on `lookup i g2 = lookup i g1` >> fs[])
+  >- (qcase_tac `known exps as g0 = (al1,g1)` >>
+      Cases_on `i ∈ domain g1` >> fs[] >>
+      Cases_on `i ∈ domain g0` >> fs[] >>
+      Cases_on `lookup i g1 = lookup i g0` >> fs[])
+  >- (qcase_tac `known _ _  g0 = (al1,g1)` >>
+      Cases_on `i ∈ domain g1` >> fs[] >>
+      Cases_on `i ∈ domain g0` >> fs[] >>
+      Cases_on `lookup i g1 = lookup i g0` >> fs[])
+  >- (qcase_tac `known _ _  g0 = (_,g1)` >>
+      qcase_tac `known_op opn` >>
+      Cases_on `i ∈ domain g1` >> fs[]
+      >- (Cases_on `i ∈ domain g0` >> fs[] >>
+          Cases_on `lookup i g1 = lookup i g0` >> fs[] >>
+          Cases_on `opn` >> fs[known_op_def, eqs, op_gbag_def] >> rveq >>
+          fs[]
+          >- fs[lookup_insert, bool_case_eq]
+          >- fs[lookup_insert, bool_case_eq]
+          >- (fs[va_case_eq, eqs, bool_case_eq] >> rveq >> fs[])) >>
+      Cases_on `opn` >>
+      fs[known_op_def, eqs, op_gbag_def, va_case_eq, bool_case_eq] >> rveq >>
+      fs[])
+  >- (qcase_tac `known _ _ g0 = (_, g1)` >>
+      Cases_on `i ∈ domain g1` >> fs[] >>
+      Cases_on `lookup i g1 = lookup i g0` >> fs[] >>
+      Cases_on `lookup i g = lookup i g1` >> fs[])
+  >- simp[Once foldr_bu'])
 
 val subspt_def = Define`
   subspt sp1 sp2 ⇔
@@ -200,6 +346,23 @@ val subspt_better_definedg = Q.store_thm(
   `v3 = v1` by metis_tac[SOME_11] >> rveq >>
   `v1 ◁ v2 ∧ v2 ◁ v1` by metis_tac[THE_DEF] >>
   metis_tac[subapprox_antisym])
+
+val subspt_known_elist_globals = Q.store_thm(
+  "subspt_known_elist_globals",
+  `known es1 as1 g0 = (al1, g1) ∧ known es2 as2 g1 = (al2, g2) ∧ subspt g0 g2 ∧
+   BAG_DISJOINT (elist_globals es1) (elist_globals es2) ⇒
+   subspt g0 g1 ∧ subspt g1 g2`,
+  strip_tac >>
+  `subspt g0 g1` by metis_tac[known_better_definedg, subspt_better_definedg] >>
+  simp[] >> fs[subspt_def] >>
+  rpt (gen_tac ORELSE disch_then strip_assume_tac) >>
+  `better_definedg g1 g2` by metis_tac[known_better_definedg] >>
+  `k ∈ domain g2` by fs[better_definedg_def] >> simp[] >>
+  spose_not_then strip_assume_tac >>
+  `k ∈ SET_OF_BAG (elist_globals es2)` by metis_tac[known_changed_globals] >>
+  Cases_on `k ∈ domain g0` >- metis_tac[] >>
+  `k ∈ SET_OF_BAG (elist_globals es1)` by metis_tac[known_changed_globals] >>
+  fs[BAG_DISJOINT, DISJOINT_DEF, EXTENSION] >> metis_tac[])
 
 (*
 val safe_setglobals_known_fixed_union = Q.store_thm(
@@ -268,11 +431,6 @@ val safe_setglobals_known_subspt = Q.store_thm(
 
 *)
 
-val op_gbag_def = Define`
-  op_gbag (SetGlobal n) = BAG_INSERT n {||} ∧
-  op_gbag _ = {||}
-`;
-
 val opn_fresh_gbag = Q.store_thm(
   "opn_fresh_gbag",
   `opn_fresh opn g ⇔ DISJOINT (SET_OF_BAG (op_gbag opn)) (domain g)`,
@@ -286,58 +444,7 @@ val known_op_adds_gbag = Q.store_thm(
   Cases_on `opn` >> dsimp[known_op_def, op_gbag_def, eqs, va_case_eq] >> rw[] >>
   simp[domain_insert]);
 
-val set_globals_def = tDefine "set_globals" `
-  (set_globals (Var _) = {||}) ∧
-  (set_globals (If e1 e2 e3) =
-    set_globals e1 ⊎ set_globals e2 ⊎ set_globals e3) ∧
-  (set_globals (Let binds e) =
-    FOLDR $BAG_UNION (set_globals e) (MAP set_globals binds)) ∧
-  (set_globals (Raise e) = set_globals e) ∧
-  (set_globals (Handle e1 e2) = set_globals e1 ⊎ set_globals e2) ∧
-  (set_globals (Tick e) = set_globals e) ∧
-  (set_globals (Call _ args) = FOLDR $BAG_UNION {||} (MAP set_globals args)) ∧
-  (set_globals (App _ f args) =
-    FOLDR $BAG_UNION (set_globals f) (MAP set_globals args)) ∧
-  (set_globals (Fn _ _ _ bod) = set_globals bod) ∧
-  (set_globals (Letrec _ _ fbinds bod) =
-    FOLDR (λne s. set_globals (SND ne) ⊎ s) (set_globals bod) fbinds) ∧
-  (set_globals (Op opn args) =
-    FOLDR $BAG_UNION (op_gbag opn) (MAP set_globals args))
-`
-  (WF_REL_TAC `measure exp_size` >> simp[] >> rpt strip_tac >>
-   imp_res_tac exp_size_MEM >> simp[])
 
-val elist_globals_def = Define`
-  elist_globals es = FOLDR BAG_UNION {||} (MAP set_globals es)
-`;
-val elist_globals_thm = Q.store_thm(
-  "elist_globals_thm[simp]",
-  `elist_globals [] = {||} ∧
-   elist_globals (exp::rest) = set_globals exp ⊎ elist_globals rest`,
-  simp[elist_globals_def]);
-val FOLDR_BAG_UNION_extract_acc = Q.store_thm(
-  "FOLDR_BAG_UNION_extract_acc",
-  `∀l a b. a ⊎ FOLDR (BAG_UNION o f) b l = FOLDR (BAG_UNION o f) (a ⊎ b) l`,
-  Induct_on `l` >> simp[] >> metis_tac[COMM_BAG_UNION, ASSOC_BAG_UNION])
-
-val foldr_bu =
-    FOLDR_BAG_UNION_extract_acc |> SPEC_ALL
-                                |> INST_TYPE [alpha |-> ``:β bag``]
-                                |> Q.INST [`b` |-> `{||}`, `f` |-> `I`]
-                                |> SIMP_RULE (srw_ss()) []
-                                |> GSYM
-
-val foldr_bu' =
-    FOLDR_BAG_UNION_extract_acc |> SPEC_ALL
-                                |> Q.INST [`b` |-> `{||}`, `f` |-> `λa. g a`]
-                                |> SIMP_RULE (srw_ss()) [o_ABS_R]
-                                |> GSYM
-
-
-val set_globals_def = save_thm("set_globals_def[simp]",
-  set_globals_def |> ONCE_REWRITE_RULE [foldr_bu]
-                  |> SIMP_RULE (srw_ss() ++ ETA_ss) [GSYM elist_globals_def])
-val set_globals_ind = theorem "set_globals_ind"
 
 val FINITE_BAG_FOLDR = Q.store_thm(
   "FINITE_BAG_FOLDR",
@@ -965,18 +1072,21 @@ val ssgc_free_preserved_SING = Q.store_thm(
 val known_op_correct_approx = Q.store_thm(
   "known_op_correct_approx",
   `known_op opn args g0 = (a,g) ∧ LIST_REL val_approx_val args vs ∧
-   state_globals_approx s0 g0 ∧
+   subspt g g' ∧
+   state_globals_approx s0 g' ∧
    do_app opn vs s0 = Rval (v, s) ⇒
-   state_globals_approx s g ∧ val_approx_val a v`,
+   state_globals_approx s g' ∧ val_approx_val a v`,
   Cases_on `opn` >>
   simp[known_op_def, do_app_def, eqs, va_case_eq, bool_case_eq,
        pair_case_eq] >>
   rpt strip_tac >> rveq >> fs[]
-  >- (fs[state_globals_approx_def] >> metis_tac[SOME_11])
+  >- (fs[state_globals_approx_def] >> res_tac >>
+      fs[subspt_def] >> metis_tac[SOME_11, domain_lookup])
   >- (fs[state_globals_approx_def, get_global_def, EL_LUPDATE,
-         lookup_insert, bool_case_eq] >> rw[] >> simp[] >> metis_tac[])
+         lookup_insert, bool_case_eq] >> rw[] >> simp[] >>
+      fs[subspt_def])
   >- (fs[state_globals_approx_def, get_global_def, EL_LUPDATE,
-         bool_case_eq, lookup_insert] >> rw[] >>
+         bool_case_eq, lookup_insert] >> rw[] >> fs[subspt_def] >>
       metis_tac[val_approx_val_merge_I])
   >- (fs[state_globals_approx_def, get_global_def, EL_APPEND_EQN,
          bool_case_eq] >> rw[]
@@ -986,18 +1096,27 @@ val known_op_correct_approx = Q.store_thm(
           pop_assum (fn th => fs[th])))
   >- (rveq >> fs[LIST_REL_EL_EQN]));
 
+val known_CONS = Q.store_thm(
+  "known_CONS",
+  `known (e::es) as g0 =
+    let (al1,g') = known [e] as g0 in
+    let (all,g) = known es as g'
+    in
+       (al1 ++ all, g)`,
+  Cases_on `es` >> simp[known_def] >> pairarg_tac >> simp[]);
+
+(*
 val say = say0 "known_correct_approx"
 val known_correct_approx = Q.store_thm(
   "known_correct_approx",
-  `∀es as g0 all g.
-     known es as g0 = (all,g) ⇒
-     ∀env s0 s vs result.
-        LIST_REL val_approx_val as env ∧
-        state_globals_approx s0 g ∧ ssgc_free s0 ∧ EVERY vsgc_free env ∧
-        EVERY esgc_free es ∧
-        evaluate(MAP FST all, env, s0) = (result, s) ⇒
-        state_globals_approx s g ∧
-        ∀vs. result = Rval vs ⇒ LIST_REL val_approx_val (MAP SND all) vs`,
+  `∀es as g0 all g env s0 s result g'.
+     known es as g0 = (all,g) ∧ BAG_ALL_DISTINCT (elist_globals es) ∧
+     LIST_REL val_approx_val as env ∧ subspt g0 g ∧ subspt g g' ∧
+     state_globals_approx s0 g' ∧ ssgc_free s0 ∧ EVERY vsgc_free env ∧
+     EVERY esgc_free es ∧ evaluate(MAP FST all, env, s0) = (result, s)
+    ⇒
+     state_globals_approx s g' ∧
+     ∀vs. result = Rval vs ⇒ LIST_REL val_approx_val (MAP SND all) vs`,
   ho_match_mp_tac known_ind >> simp[known_def] >>
   rpt conj_tac >> rpt (gen_tac ORELSE disch_then strip_assume_tac)
   >- (* nil *) (say "nil" >> fs[evaluate_def] >> rw[])
@@ -1013,33 +1132,50 @@ val known_correct_approx = Q.store_thm(
         by (Cases_on `al2` >> fs[] >> metis_tac[pair_CASES]) >> rveq >>
       fs[evaluate_def, pair_case_eq, result_case_eq] >> rveq
       >- (qcase_tac `evaluate ([exp1'], env, s0) = (Rval v1, s1)` >>
-          first_x_assum (fn th =>
-            qspecl_then [`env`, `s0`, `s1`, `Rval v1`] mp_tac th >>
-            simp[] >>
-            disch_then (CONJUNCTS_THEN strip_assume_tac)) >>
-          rveq >> fs[] >>
-          qcase_tac `evaluate(_::_, env, s1) = (Rval vs, s)` >>
-          `ssgc_free s1` by metis_tac[ssgc_free_preserved_SING] >>
-          first_x_assum (qspecl_then [`env`, `s1`, `s`, `Rval vs`] mp_tac) >>
-          simp[])
-      >- (simp[] >>
-          qcase_tac `evaluate ([exp1'], env, s0) = (Rval v1, s1)` >>
-          first_x_assum (fn th =>
-            qspecl_then [`env`, `s0`, `s1`, `Rval v1`] mp_tac th >>
-            simp[] >>
-            disch_then (CONJUNCTS_THEN strip_assume_tac)) >>
-          `ssgc_free s1` suffices_by metis_tac[] >>
-          metis_tac[ssgc_free_preserved_SING])
-      >- (simp[] >>
-          qcase_tac `evaluate ([exp1'], env, s0) = (Rerr error, s1)` >>
-          first_x_assum (qspecl_then [`env`, `s0`, `s1`, `Rerr error`] mp_tac)>>
+          qpat_assum `closSem$evaluate([_],_,_) = _` (fn th =>
+            first_x_assum (fn ith =>
+              mp_tac (asmPART_MATCH' last ith (concl th))) >> assume_tac th) >>
           simp[] >>
-          metis_tac[known_better_definedg, state_approx_better_definedg]))
+          disch_then (resolve_selected last) >> simp[] >>
+          fs[BAG_ALL_DISTINCT_BAG_UNION] >>
+          `subspt g0 g1 ∧ subspt g1 g`
+            by first_assum (fn kth2 =>
+                  first_assum (fn kth1 => mp_tac
+                            (asmPART_MATCH' hd
+                                            (GEN_ALL subspt_known_elist_globals)
+                                            (concl kth1))) >>
+                  simp[] >> disch_then (resolve_selected hd) >> simp[]) >>
+          simp[] >> impl_keep_tac >- metis_tac[subspt_trans] >> strip_tac >>
+          rveq >> fs[] >> sel_ihpc last >> simp[] >>
+          metis_tac[ssgc_free_preserved_SING])
+      >- (simp[] >> fs[BAG_ALL_DISTINCT_BAG_UNION] >>
+          qpat_assum `closSem$evaluate ([_],_,_) = _` (fn th =>
+            first_x_assum (fn ith =>
+              mp_tac (asmPART_MATCH' last ith (concl th))) >> assume_tac th) >>
+          simp[] >>
+          disch_then (resolve_selected last) >> simp[] >>
+          first_assum (fn kth2 =>
+                  first_assum (fn kth1 => mp_tac
+                            (asmPART_MATCH' hd
+                                            (GEN_ALL subspt_known_elist_globals)
+                                            (concl kth1))) >>
+                  simp[] >> disch_then (resolve_selected hd) >> simp[]) >>
+          strip_tac >> impl_tac >- metis_tac[subspt_trans] >> rw[] >>
+          sel_ihpc last >> simp[] >> disch_then irule >> simp[]>>
+          metis_tac[ssgc_free_preserved_SING])
+      >- (simp[] >> sel_ihpc last >> simp[] >> fs[BAG_ALL_DISTINCT_BAG_UNION] >>
+          first_assum (fn kth2 =>
+                  first_assum (fn kth1 => mp_tac
+                            (asmPART_MATCH' hd
+                                            (GEN_ALL subspt_known_elist_globals)
+                                            (concl kth1))) >>
+                  simp[] >> disch_then (resolve_selected hd) >> simp[]) >>
+          metis_tac[subspt_trans]))
   >- ((* Var *) say "var" >>
       fs[any_el_ALT, evaluate_def, bool_case_eq] >>
       fs[LIST_REL_EL_EQN])
   >- ((* If *) say "if" >>
-      rpt (pairarg_tac >> fs[]) >> rveq >> fs[] >>
+      rpt (pairarg_tac >> fs[]) >> rveq >> fs[BAG_ALL_DISTINCT_BAG_UNION] >>
       qcase_tac `known [ge] as g0 = (_, g1)` >>
       `∃ge' apx1. known [ge] as g0 = ([(ge',apx1)], g1)`
          by metis_tac[known_sing, PAIR_EQ] >>
@@ -1049,51 +1185,55 @@ val known_correct_approx = Q.store_thm(
       qcase_tac `known [eb] as g2 = (_, g3)` >>
       `∃eb' apx3. known [eb] as g2 = ([(eb',apx3)], g3)`
          by metis_tac[known_sing, PAIR_EQ] >> fs[] >> rveq >> fs[] >> rveq >>
+      `subspt g0 g1 ∧ subspt g1 g2 ∧ subspt g2 g3`
+         by (`∃al01. known [ge;tb] as g0 = (al01,g2)` by simp[known_def] >>
+             first_assum (fn th =>
+               mp_tac (asmPART_MATCH' hd (GEN_ALL subspt_known_elist_globals)
+                                      (concl th))) >> simp[] >>
+             disch_then (resolve_selected hd) >> simp[] >> strip_tac >>
+             qpat_assum `known [_] _ g0 = (_,g1)` (fn th =>
+               mp_tac (asmPART_MATCH' hd (GEN_ALL subspt_known_elist_globals)
+                                      (concl th)) >> assume_tac th) >>
+             simp[] >> disch_then (resolve_selected hd) >> simp[]) >>
       reverse
         (fs[evaluate_def, pair_case_eq, result_case_eq,
             bool_case_eq]) >> rveq >> fixeqs >> simp[]
-      >- metis_tac[known_better_definedg, state_approx_better_definedg]
-      >- metis_tac[known_better_definedg, state_approx_better_definedg] >>
+      >- (sel_ihpc last >> simp[] >> metis_tac[subspt_trans])
+      >- (sel_ihpc last >> simp[] >> metis_tac[subspt_trans]) >>
       (* two cases from here on *)
       qcase_tac `evaluate ([ge'], env, s0) = (Rval gvs, s1)` >>
-      first_x_assum
-       (fn th => qspecl_then [`env`, `s0`, `s1`, `Rval gvs`] mp_tac th >>
-                 simp[] >>
-                 disch_then (CONJUNCTS_THEN strip_assume_tac)) >>
-      rveq >> fs[] >> rveq >>
-      qcase_tac `evaluate ([somebr], env, s1) = (someres, s2)` >>
-      `state_globals_approx s1 g2`
-        by metis_tac[known_better_definedg, state_approx_better_definedg] >>
-      `ssgc_free s1` by metis_tac[ssgc_free_preserved_SING] >>
-      first_x_assum
-       (fn th => qspecl_then [`env`, `s1`, `s2`, `someres`] mp_tac th >>
-                 simp[] >>
-                 disch_then (CONJUNCTS_THEN strip_assume_tac)) >>
-      metis_tac[val_approx_val_merge_I, known_better_definedg,
-                state_approx_better_definedg])
+      qpat_assum `evaluate ([ge'], _, _) = _` (fn th =>
+        first_x_assum (fn ith =>
+          mp_tac (asmPART_MATCH' last ith (concl th))) >> assume_tac th) >>
+      simp[] >> disch_then (resolve_selected last) >> simp[] >>
+      (impl_keep_tac >- metis_tac[subspt_trans]) >>
+      strip_tac >> rveq >> fs[] >> rveq >> sel_ihpc last >> simp[] >>
+      disch_then (resolve_selected (el 2)) >> simp[] >>
+      impl_tac
+      >- metis_tac[ssgc_free_preserved_SING]
+      >- metis_tac[val_approx_val_merge_I]
+      >- (conj_tac >- metis_tac[subspt_trans] >>
+          irule (GEN_ALL ssgc_free_preserved_SING) >> metis_tac[])
+      >- metis_tac[val_approx_val_merge_I])
   >- ((* let *) say "let" >>
       rpt (pairarg_tac >> fs[]) >> rveq >> fs[] >>
       fs[evaluate_def, eqs, pair_case_eq, result_case_eq] >>
-      rveq
-      >- (qcase_tac `evaluate (MAP FST binds', env, s0) = (Rval bvs, s1)` >>
-          first_x_assum
-            (fn th => qspecl_then [`env`, `s0`, `s1`, `Rval bvs`] mp_tac th >>
-                      simp[] >> disch_then (CONJUNCTS_THEN assume_tac)) >>
-          qcase_tac `evaluate ([bod'], bvs ++ env, s1) = (result, s)` >>
-          qspecl_then [`MAP FST binds'`, `env`, `s0`, `Rval bvs`, `s1`]
-                      mp_tac ssgc_evaluate >> simp[] >> impl_tac
-          >- (simp[ALL_EL_MAP] >> metis_tac [known_preserves_esgc_free]) >>
-          strip_tac >> imp_res_tac known_sing_EQ_E >> fs[] >> rveq >>
-          first_x_assum
-            (qspecl_then [`bvs ++ env`, `s1`, `s`, `result`] mp_tac) >>
-          simp[EVERY2_APPEND_suff])
-      >- (qcase_tac `evaluate (MAP FST binds',env,s0) = (Rerr err, s)` >>
-          first_x_assum
-            (fn th =>
-               qspecl_then [`env`, `s0`, `s`, `Rerr err`] mp_tac th >>
-               simp[] >>
-               disch_then (assume_tac o assert (not o is_imp o concl))) >>
-          metis_tac[state_approx_better_definedg, known_better_definedg]))
+      rveq >> sel_ihpc last >> simp[] >> disch_then (resolve_selected last) >>
+      simp[] >> fs[BAG_ALL_DISTINCT_BAG_UNION] >>
+      map_every qcase_tac [`known [bod] _ g1 = (_, g)`,
+                           `known _ _ g0 = (_, g1)`] >>
+      qpat_assum `known [_] _ _ = _` (fn th =>
+        mp_tac (asmPART_MATCH' (el 2) (GEN_ALL subspt_known_elist_globals)
+                               (concl th)) >> assume_tac th) >> simp[] >>
+      disch_then (resolve_selected hd) >> simp[] >>
+      (impl_tac >- fs[BAG_DISJOINT, DISJOINT_SYM]) >> strip_tac >> simp[] >>
+      (impl_tac >- metis_tac[subspt_trans]) >> strip_tac >> simp[] >>
+      imp_res_tac known_sing_EQ_E >> rveq >> fs[] >> rveq >>
+      sel_ihpc last >> simp[EVERY2_APPEND_suff] >>
+      disch_then (resolve_selected (el 2)) >> simp[] >> reverse impl_tac
+      >- rw[] >> resolve_selected hd ssgc_evaluate >> simp[] >>
+      disch_then (resolve_selected last) >> simp[] >>
+      imp_res_tac known_preserves_esgc_free >> simp[ALL_EL_MAP])
   >- ((* raise *) say "raise" >>
       pairarg_tac >> fs[] >> imp_res_tac known_sing_EQ_E >> fs[] >> rveq >>
       fs[evaluate_def, pair_case_eq, result_case_eq] >> rveq >>
@@ -1101,82 +1241,76 @@ val known_correct_approx = Q.store_thm(
   >- ((* tick *) say "tick" >>
       pairarg_tac >> fs[] >> imp_res_tac known_sing_EQ_E >> fs[] >> rveq >>
       fs[evaluate_def, pair_case_eq, result_case_eq,
-         bool_case_eq] >> rveq >> simp[]
-      >- metis_tac[state_approx_better_definedg, known_better_definedg] >>
-      fixeqs >> first_x_assum irule >>
-      map_every qexists_tac [`env`, `dec_clock 1 s0`] >> simp[])
+         bool_case_eq] >> rveq >> simp[] >>
+      fixeqs >> first_x_assum irule >> simp[] >>
+      metis_tac[state_globals_approx_dec_clock, ssgc_free_dec_clock])
   >- ((* handle *) say "handle" >>
       rpt (pairarg_tac >> fs[]) >> rveq >> fs[] >>
+      map_every qcase_tac [`known _ (_ :: _) g1 = (_, g)`,
+                           `known _ _ g0 = (_, g1)`] >>
+      qpat_assum `known _ (_ :: _) _ = _` (fn th =>
+        mp_tac (asmPART_MATCH' (el 2) (GEN_ALL subspt_known_elist_globals)
+                               (concl th)) >> assume_tac th) >> simp[] >>
+      disch_then (resolve_selected hd) >> simp[] >>
+      fs[BAG_ALL_DISTINCT_BAG_UNION] >> strip_tac >>
       fs[evaluate_def, pair_case_eq, result_case_eq,
-         error_case_eq] >> rveq >> fs[]
-      >- (imp_res_tac known_sing_EQ_E >> rveq >> fs[] >> rveq >>
-          qcase_tac `evaluate([e1],env,s0) = (Rval vs,s)` >>
-          first_x_assum
-            (fn th => qspecl_then [`env`, `s0`, `s`, `Rval vs`] mp_tac th >>
-                      simp[] >> disch_then (CONJUNCTS_THEN strip_assume_tac)) >>
-          fs[] >> metis_tac[val_approx_val_merge_I, known_better_definedg,
-                            state_approx_better_definedg])
-      >- (imp_res_tac known_sing_EQ_E >> rveq >> fs[] >> rveq >>
-          qcase_tac `evaluate([exp1],env,s0) = (Rerr(Rraise exc),s1)` >>
-          first_x_assum
-            (fn th => qspecl_then [`env`, `s0`, `s1`, `Rerr (Rraise exc)`]
-                                  mp_tac th >> simp[] >>
-                      disch_then
-                        (assume_tac o assert (not o is_imp o concl))) >>
-          qcase_tac `evaluate([hnd],exc::env,s1) = (result,s)` >>
-          first_x_assum (qspecl_then [`exc::env`, `s1`, `s`, `result`] mp_tac)>>
-          simp[] >>
-          qspecl_then [`[exp1]`, `env`, `s0`, `Rerr (Rraise exc)`, `s1`]
-                      mp_tac ssgc_evaluate >> simp[] >> impl_tac
-          >- (qcase_tac `known [exp0] as g0 = ([(exp1,_)], _)` >>
-              qspecl_then [`[exp0]`, `as`] mp_tac known_preserves_esgc_free >>
-              disch_then (IMP_RES_THEN mp_tac) >> simp[]) >> simp[] >>
-          rpt strip_tac >> simp[] >> fs[] >> metis_tac[val_approx_val_merge_I])
-      >- (imp_res_tac known_sing_EQ_E >> rveq >> fs[] >> rveq >>
-          qcase_tac `evaluate([exp1],env,s0) = (Rerr (Rabort abt), s)` >>
-          first_x_assum
-            (fn th => qspecl_then [`env`, `s0`, `s`, `Rerr (Rabort abt)`]
-                                  mp_tac th >> simp[] >>
-                      disch_then
-                        (assume_tac o assert (not o is_imp o concl))) >>
-          metis_tac[known_better_definedg, state_approx_better_definedg]))
+         error_case_eq] >> rveq >> fs[] >>
+      imp_res_tac known_sing_EQ_E >> rveq >> fs[] >> rveq
+      >- (sel_ihpc last >> simp[] >> disch_then (resolve_selected last) >>
+          simp[] >> reverse impl_keep_tac
+          >- metis_tac[val_approx_val_merge_I] >>
+          metis_tac[subspt_trans])
+      >- (qpat_assum `closSem$evaluate _ = (Rerr _, _)`
+           (fn th => first_x_assum (fn ith =>
+              mp_tac (asmPART_MATCH' last ith (concl th))) >> assume_tac th) >>
+          simp[] >> disch_then (resolve_selected last) >> simp[] >>
+          impl_keep_tac >- metis_tac[subspt_trans] >>
+          strip_tac >> sel_ihpc last >> simp[PULL_EXISTS] >>
+          disch_then (resolve_selected (el 2)) >> simp[] >> reverse impl_tac
+          >- metis_tac[val_approx_val_merge_I] >>
+          conj_tac >- metis_tac[ssgc_free_preserved_SING] >>
+          resolve_selected hd ssgc_evaluate >>
+          disch_then (resolve_selected last) >> simp[] >> reverse impl_tac
+          >- simp[] >>
+          imp_res_tac known_preserves_esgc_free >> fs[])
+      >- (sel_ihpc last >> simp[] >> metis_tac[subspt_trans]))
   >- ((* call *) say "call" >> pairarg_tac >> fs[] >> rveq >> fs[] >>
       fs[evaluate_def, pair_case_eq, result_case_eq, eqs,
          bool_case_eq] >>
-      rveq >> fs[]
-      >- (qcase_tac `evaluate(MAP FST args,env,s0) = (Rval vs, s)` >>
-          first_x_assum (qspecl_then [`env`, `s0`, `s`, `Rval vs`] mp_tac) >>
-          simp[])
-      >- (qcase_tac `evaluate(MAP FST arg_es,env,s0) = (Rval vs, s)` >>
-          first_x_assum (qspecl_then [`env`, `s0`, `s`, `Rval vs`] mp_tac) >>
-          simp[])
-      >- (fixeqs >>
-          qcase_tac `evaluate(MAP FST arg_es, env, s0) = (Rval vs, s1)` >>
-          first_x_assum (qspecl_then [`env`, `s0`, `s1`, `Rval vs`] mp_tac) >>
-          simp[] >> rw[]
-          >- (qcase_tac `evaluate([body],args,dec_clock 1 s1) = (result,s)` >>
-              qspecl_then [`MAP FST arg_es`, `env`, `s0`, `Rval vs`, `s1`]
-                          mp_tac ssgc_evaluate >> simp[] >>
-              impl_tac
-              >- (simp[ALL_EL_MAP] >> metis_tac[known_preserves_esgc_free]) >>
-              rw[] >>
-              qspecl_then [`[body]`, `args`, `dec_clock 1 s1`, `result`, `s`]
-                          mp_tac ssgc_evaluate >> simp[] >>
-              fs[find_code_def, eqs, pair_case_eq] >> rveq >>
-              simp[] >>
-              `set_globals body = {||}`
-                by (Q.UNDISCH_THEN `ssgc_free s1` mp_tac >>
-                    simp[ssgc_free_def] >> metis_tac[])  >>
-              simp[set_globals_empty_esgc_free] >> strip_tac >>
-              `mapped_globals s1 ⊆ mapped_globals s`
-                by metis_tac[mapped_globals_grow, mapped_globals_dec_clock] >>
-              metis_tac[mglobals_extend_EMPTY_state_globals_approx])
-          >- metis_tac[evaluate_SING])
-      >- (qcase_tac `evaluate(MAP FST arg_es,env,s0) = (Rerr err, s)` >>
-          first_x_assum (qspecl_then [`env`, `s0`] mp_tac) >> simp[]))
+      rveq >> fs[] >> sel_ihpc last >> simp[] >> fixeqs >>
+      disch_then (resolve_selected last) >> simp[] >>
+      reverse (rpt strip_tac)
+      >- (rveq >> imp_res_tac evaluate_SING >> simp[]) >>
+      map_every qcase_tac [
+        `evaluate([body],args,dec_clock 1 s1) = (result,s)`,
+        `evaluate(MAP FST alist,env,s0) = (Rval vs, s1)`] >>
+      `ssgc_free s1 ∧ EVERY vsgc_free vs`
+         by (resolve_selected hd ssgc_evaluate >> simp[] >>
+             disch_then (resolve_selected last) >> simp[] >>
+             reverse impl_tac >- simp[] >>
+             imp_res_tac known_preserves_esgc_free >> simp[ALL_EL_MAP]) >>
+      `set_globals body = {||}`
+         by (Q.UNDISCH_THEN `ssgc_free s1` mp_tac >>
+             simp[ssgc_free_def] >> fs[find_code_def, eqs, pair_case_eq] >>
+             metis_tac[])  >>
+      `mapped_globals s1 ⊆ mapped_globals s`
+         by metis_tac[mapped_globals_grow, mapped_globals_dec_clock] >>
+      `mglobals_extend s1 {} s`
+         by (qspecl_then [`[body]`, `args`, `dec_clock 1 s1`, `result`, `s`]
+                         mp_tac ssgc_evaluate >> simp[] >>
+             fs[find_code_def, eqs, pair_case_eq] >> rveq >>
+             simp[set_globals_empty_esgc_free]) >>
+      metis_tac[mglobals_extend_EMPTY_state_globals_approx])
   >- ((* op *) say "op" >> rpt (pairarg_tac >> fs[]) >> rveq >> fs[] >>
+      fs[BAG_ALL_DISTINCT_BAG_UNION]
+subspt_better_definedg
       fs[evaluate_def, pair_case_eq, result_case_eq] >> rveq >>
-      fs[] >>
+      fs[] >> sel_ihpc last >> simp[] >> disch_then (resolve_selected last) >>
+      simp[] >>
+      (impl_keep_tac
+       >- metis_tac[known_op_better_definedg, better_definedg_trans]) >>
+      simp[]
+
       qcase_tac `evaluate(MAP FST args,env,s0)` >>
       first_x_assum (qspecl_then [`env`, `s0`] mp_tac) >> simp[]
       >- metis_tac[known_op_correct_approx, LIST_REL_REVERSE_EQ] >>
@@ -1299,63 +1433,6 @@ val ssgc_free_preserved_SING' = Q.store_thm(
 
 val say = say0 "known_correct";
 
-fun nailIHx k = let
-  fun hdt t = (t |> lhs |> strip_comb |> #1)
-              handle HOL_ERR _ => t |> strip_comb |> #1
-  fun sameish t1 t2 = aconv t1 t2 orelse same_const t1 t2
-  fun samehd t1 th2 = sameish (hdt t1) (hdt (concl th2))
-  fun findcs [] a k = raise Fail "strip_conj gave empty list"
-    | findcs [c] a k =
-      first_assum
-        (fn th => k (LIST_CONJ (List.rev (assert (samehd c) th :: a))))
-    | findcs (c::cs) a k =
-      first_assum (fn th => findcs cs (assert (samehd c) th :: a) k)
-in
-  first_x_assum
-    (fn th0 =>
-        let val body = th0 |> concl |> strip_forall |> #2
-            val hyp = #1 (dest_imp body)
-            val cs = strip_conj hyp
-        in
-          findcs cs [] (k o MATCH_MP th0)
-        end)
-end
-
-fun avSPEC_ALL avds th =
-  let
-    fun recurse avds acc th =
-      case Lib.total dest_forall (concl th) of
-          SOME (v,bod) =>
-          let
-            val v' = variant avds v
-          in
-            recurse (v'::avds) (v'::acc) (SPEC v' th)
-          end
-        | NONE => (List.rev acc, th)
-  in
-    recurse avds [] th
-  end
-
-fun PART_MATCH' f th t =
-  let
-    val (vs, _) = strip_forall (concl th)
-    val hypfvs_set = hyp_frees th
-    val hypfvs = HOLset.listItems hypfvs_set
-    val tfvs = free_vars t
-    val dontspec = union tfvs hypfvs
-    val (vs, speccedth) = avSPEC_ALL dontspec th
-    val ((tmsig,_),_) = raw_match [] hypfvs_set (f (concl speccedth)) t ([],[])
-    val dontgen = union (map #redex tmsig) dontspec
-  in
-    GENL (set_diff vs dontgen) (INST tmsig speccedth)
-  end
-
-fun asmPART_MATCH' f th t =
-    PART_MATCH' (f o strip_conj o #1 o dest_imp) th t
-
-fun sel_ihpc f =
-    first_assum (fn asm => first_x_assum (fn ih =>
-      mp_tac (asmPART_MATCH' f ih (concl asm))))
 
 val evaluate_app_NONE_SOME = Q.store_thm(
   "evaluate_app_NONE_SOME",
@@ -1374,8 +1451,8 @@ val evaluate_app_NONE_SOME = Q.store_thm(
   fs[check_loc_def, revdroprev, revtakerev]);
 
 val kerel_def = Define`
-  kerel as g0 e1 e2 ⇔
-    ∃g0' g apx. better_definedg g0' g0 ∧ known [e1] as g0' = ([(e2,apx)], g)
+  kerel as g' e1 e2 ⇔
+    ∃g0 g apx. better_definedg g g' ∧ known [e1] as g0 = ([(e2,apx)], g)
 `;
 
 val kvrel_def = tDefine "kvrel" `
@@ -1867,14 +1944,14 @@ val krrel_better_definedg = Q.store_thm(
   Cases_on `res1` >> simp[krrel_err_rw] >>
   metis_tac[kvrel_LIST_REL_better_definedg, ksrel_better_definedg,
             kvrel_better_definedg]);
-(*
+
 val known_correct0 = Q.prove(
   `(∀a es env1 env2 (s01:α closSem$state) s02 res1 s1 g0 g g' as ealist.
       a = (es,env1,s01) ∧ evaluate (es, env1, s01) = (res1, s1) ∧
       EVERY esgc_free es ∧ better_definedg g g' ∧
       LIST_REL val_approx_val as env1 ∧ EVERY vsgc_free env1 ∧
       LIST_REL (kvrel g') env1 env2 ∧ ksrel g' s01 s02 ∧
-      state_globals_approx s01 g0 ∧
+      state_globals_approx s01 g' ∧
       ssgc_free s01 ∧ known es as g0 = (ealist, g) ⇒
       ∃res2 s2.
         evaluate(MAP FST ealist, env2, s02) = (res2, s2) ∧
@@ -1882,7 +1959,7 @@ val known_correct0 = Q.prove(
    (∀lopt1 f1 args1 (s01:α closSem$state) res1 s1 lopt2 f2 args2 s02 g.
       evaluate_app lopt1 f1 args1 s01 = (res1,s1) ∧ ssgc_free s01 ∧
       kvrel g f1 f2 ∧ LIST_REL (kvrel g) args1 args2 ∧
-      ksrel g s01 s02 ∧
+      ksrel g s01 s02 ∧ state_globals_approx s01 g ∧
       EVERY vsgc_free args1 ∧ loptrel f2 (LENGTH args1) lopt1 lopt2 ⇒
       ∃res2 s2.
         evaluate_app lopt2 f2 args2 s02 = (res2,s2) ∧
@@ -1907,7 +1984,8 @@ val known_correct0 = Q.prove(
             disch_then
               (fn impth => mp_tac (asmPART_MATCH' last impth (concl th)))) >>
       simp[] >> impl_keep_tac
-      >- metis_tac[known_better_definedg, better_definedg_trans] >> rw[]
+      >- metis_tac[known_better_definedg, better_definedg_trans] >>
+      rw[]
       >- (imp_res_tac known_sing_EQ_E >> rveq >> fs[] >>
           sel_ihpc last >> simp[] >> strip_tac >>
           sel_ihpc (el 3) >> simp[] >> strip_tac >>
@@ -2088,19 +2166,27 @@ val known_correct0 = Q.prove(
       simp[evaluate_def, pair_case_eq, result_case_eq,
            error_case_eq, known_def] >> rpt strip_tac >> rveq >> fs[] >>
       rpt (pairarg_tac >> fs[]) >> rveq >>
-      imp_res_tac known_sing_EQ_E >> rveq >> fs[] >> rveq >>
-      nailIHx strip_assume_tac >> fs[] >>
-      simp[evaluate_def, pair_case_eq, result_case_eq, error_case_eq]
-      >- metis_tac[known_better_definedg, kvrel_LIST_REL_better_definedg,
-                   ksrel_better_definedg]
-      >- (dsimp[] >> fs[krrel_err_rw, PULL_EXISTS] >>
-          sel_ihpc last >> simp[] >> disch_then irule >> simp[]
+      imp_res_tac known_sing_EQ_E >> rveq >> fs[] >> rveq
+      >- (sel_ihpc last >> simp[] >> strip_tac >> sel_ihpc last >> simp[] >>
+          strip_tac >> sel_ihpc last >> simp[] >> impl_tac
+          >- metis_tac[known_better_definedg, better_definedg_trans] >>
+          rw[] >> simp[evaluate_def])
+      >- (dsimp[evaluate_def, pair_case_eq, result_case_eq, error_case_eq] >>
+          fs[PULL_EXISTS] >>
+          qhdtm_assum `state_globals_approx` (fn th => first_x_assum (fn ith =>
+            mp_tac (asmPART_MATCH' (el 5) ith (concl th)))) >> simp[] >>
+          rpt (disch_then (fn ith => first_assum (fn th =>
+                 mp_tac (asmPART_MATCH' last ith (concl th)))) >> simp[]) >>
+          impl_keep_tac
+          >- metis_tac[known_better_definedg, better_definedg_trans] >> rw[] >>
+          simp[] >> fs[krrel_err_rw] >> rveq >> sel_ihpc last >> simp[] >>
+          disch_then irule >> simp[]
           >- metis_tac[ssgc_free_preserved_SING']
           >- first_assum
                (fn th =>
                     mp_tac (asmPART_MATCH' last ssgc_evaluate (concl th)) >>
                     simp[] >> NO_TAC)
-          >- (qcase_tac `LIST_REL (kvrel g0) env1 env2` >> rveq >>
+          >- (qcase_tac `LIST_REL (kvrel gg) env1 env2` >> rveq >>
               qcase_tac `evaluate([exp2],env2,s02) = (Rerr (Rraise exn2),s2)` >>
               qcase_tac `known [exp1] as g0 = ([(exp2,apx1)], g0')` >>
               `state_globals_approx s2 g0'` suffices_by metis_tac[ksrel_sga] >>
@@ -2108,11 +2194,15 @@ val known_correct0 = Q.prove(
               map_every qexists_tac [`env2`, `Rerr (Rraise exn2)`, `s02`] >>
               simp[] >>
               metis_tac[ksrel_ssgc_free,kvrel_EVERY_vsgc_free,ksrel_sga,
-                        kvrel_LIST_REL_val_approx])
-         >- (metis_tac[kvrel_LIST_REL_better_definedg, known_better_definedg]))
-      >- (dsimp[] >> fs[krrel_err_rw] >>
-          metis_tac[pair_CASES, result_CASES, error_CASES,
-                    ksrel_better_definedg, known_better_definedg]))
+                        kvrel_LIST_REL_val_approx]))
+      >- (sel_ihpc last >> simp[] >>
+          rpt (disch_then (fn ith => first_assum (fn th =>
+                 mp_tac (asmPART_MATCH' last ith (concl th)))) >> simp[]) >>
+          impl_keep_tac
+          >- metis_tac[known_better_definedg, better_definedg_trans] >> rw[] >>
+          simp[evaluate_def] >>
+          fs[krrel_err_rw, result_case_eq, error_case_eq] >> dsimp[] >>
+          metis_tac[pair_CASES, result_CASES, error_CASES]))
   >- (say "op" >>
       simp[evaluate_def, pair_case_eq, result_case_eq, known_def] >>
       rpt strip_tac >> rveq >> fs[] >>
@@ -2328,7 +2418,11 @@ val known_correct0 = Q.prove(
           dsimp[] >> fs[PULL_EXISTS] >>
           map_every qcase_tac [
             `evaluate([exp1],env1,dec_clock _ s01) = (Rval [v1], s11)`,
-            `kerel envapx gg exp1 exp2`] >> fs[kerel_def] >> cheat)
+            `kerel envapx gg exp1 exp2`] >> fs[kerel_def] >>
+          rpt disj1_tac >> sel_ihpc last >> simp[] >>
+
+
+cheat)
       >- (imp_res_tac evaluate_SING >> fs[])
       >- cheat))
 
